theory/Abstract_Communication_Analysis.thy
@@ -99,5 +99,4 @@ inductive topo_pair_accept :: "topo_pair \<Rightarrow> exp \<Rightarrow> bool" (
 definition topo_accept :: "topo_env \<Rightarrow> exp \<Rightarrow> bool" (infix "\<bind>" 55) where 
   "\<A> \<bind> e \<equiv> (\<forall> x\<^sub>c . (x\<^sub>c, \<A> x\<^sub>c) \<TTurnstile> e)"
 
-
 end
